feat(*) add more examples

Zippy/Examples/Zippy_Examples.thy
@@ -2,124 +2,121 @@
 theory Zippy_Examples
   imports
     Zippy.Zippy_Prover_Instances
+    Main
 begin
 
-lemma test: "PROP A \<Longrightarrow> PROP B \<Longrightarrow> PROP G \<Longrightarrow> PROP B \<Longrightarrow> (PROP A \<Longrightarrow> PROP A) \<Longrightarrow> PROP E \<Longrightarrow> PROP A &&& PROP B &&& PROP C &&& PROP D &&& PROP E &&& PROP F &&& PROP G" sorry
+text \<open>Some simple examples showcasing navigation in the zipper and the creation of theorems using
+the best-first search instantiation from the paper.\<close>
 
-consts A :: "prop"
-consts B :: "prop"
-consts G :: "prop"
-consts E :: "prop"
-consts C :: "prop"
-consts D :: "prop"
-consts F :: "prop"
-lemmas test_inst = test[of "PROP A" "PROP B" "PROP G" "PROP E" "PROP C" "PROP D" "PROP F"]
-
-(* lemma "A \<equiv> B \<Longrightarrow> A \<equiv> C" *)
-  (* apply simp *)
-
-lemma cheat: "PROP P" sorry
-
-declare[[ML_print_depth=100]]
 ML\<open>
-  local
-    structure SC = \<^eval>\<open>sfx_ParaT_nargs "Semi_Category"\<close>(Zippy)
-    structure C = \<^eval>\<open>sfx_ParaT_nargs "Category"\<close>(Zippy)
-    structure M = \<^eval>\<open>sfx_ParaT_nargs "Monad"\<close>(Zippy.M)
-    open SC Zippy M
-  in
-    structure Zippy_DFS = \<^eval>\<open>mk_name ["DFS_Postorder_Enumerable", pfx_sfx_nargs "Alternating_Zipper"]\<close>(
-      structure Base = struct structure AE = AE end
-      structure Z =
-        \<^imap>\<open>\<open>{i}\<close> => \<open>
-        \<^eval>\<open>mk_name ["Rotate", pfx_sfx_nargs "Alternating_Zipper"]\<close>(\<close> where stop = 3\<close>
-        Zippy
-        \<^imap>\<open>\<open>{i}\<close> => \<open>)\<close> where stop = 3\<close>
-      \<^imap>\<open>\<open>{i}\<close> => \<open>
-      structure E{i} = \<^eval>\<open>sfx_T_nargs "DFS_Postorder_Enumerable_Zipper_Moves"\<close>(
-        open Base; structure Z = Z.Z{i}.ZM)\<close>\<close>
-      structure AE = AE)
-    fun halve_prio_co p = update_prio_co (fn _ => P.halve) p
-    (* val presults_from_tac = Z.presults_from_tac' @{context} *)
-    fun cheat_tac prog ctxt = resolve_tac ctxt [@{thm cheat}]
-      |> lift_all_goals_focus_tac (K (Zippy_Result_Metadata.metadata prog))
-        T.single_goal_empty_target
-    val amd = AMD.metadata (@{binding "test action"}, "action description")
-    fun add_tac amd p f tac z =
-      amd >>= (fn amd => cons_move_tac amd (halve_prio_co p) tac f z)
-    (* (halve_prio_co p) (cheat_tac mk_rmd ctxt) *)
-    fun gen_fold_run_paction_dfs fold_paction =
-      Zippy_DFS.first3 >>> fold_paction >>> fold_pactions_run_single_res
-    fun gen_fold_max_paction_dfs update_res = fold_pactions_max P.ord update_res Zippy_DFS.next
-    val test = Timing.timeit
-      (fn _ => (
-      (init_state' mk_gcd_more
-      >>> arr snd
-      >>> Down1.move
-      >>> with_state (cheat_tac RMD.unclear #> add_tac amd P.HIGH (F.goals [2]))
-      (* >>> L.get (pos1 ()) *)
-      >>> Up4.move >>> Up3.move
-      >>> with_state (cheat_tac RMD.promising #> add_tac amd P.LOW (F.goals [2]))
-      >>> Up4.move >>> Up3.move >>> Z2.ZM.Down.move
-      >>> with_state (cheat_tac RMD.unclear #> add_tac amd P.MEDIUM F.none)
-      >>> Up4.move >>> Up3.move >>> Z2.ZM.Down.move
-      >>> with_state (cheat_tac RMD.unclear #> add_tac amd P.MEDIUM F.none)
-      >>> Up4.move >>> Up3.move >>> Z2.ZM.Down.move
-      >>> with_state (cheat_tac RMD.unclear #> add_tac amd P.MEDIUM F.none)
-      >>> Up4.move >>> Up3.move >>> Up2.move >>> Z1.ZM.Unzip.move
-      >>> repeat_fold_run_max_paction_dfs_halve_prio_depth NONE
-      (* >>> Zippy_DFS.first3 *)
-      (* >>> L.get (depth4 ()) *)
-      (* >>> repeat_fold_run_max_paction_dfs_halve_prio_depth (SOME 1) *)
-      >>> Z1.ZM.Zip.move
-      >>> Down1.move
-      >>> Z2.ZM.Down.move
-      >>> Down2.move
-      >>> Down3.move
-      >>> Down4.move
-      (* >>> Down5.move *)
-      (* >>> Down1.move  *)
-      (* >>> Z2.ZM.Down.move *)
-      >>> L.get (pos5 ())
-      (* >>> Down1.move >>> Down2.move >>> Down3.move  *)
-      (* >>> repeat_fold_run_max_paction_dfs_halve_prio_depth (SOME 1) *)
-      (* >>> Z1.ZM.Unzip.move *)
-      (* >>> Zippy_DFS.first3 *)
-      (* >>> gen_fold_run_paction_dfs (gen_fold_max_paction_dfs (id ())) *)
-      (* >>> (fn z => get_run_paction z >>= (fn x => run_action x z)) *)
-      (* >>> Z1.ZM.Zip.move
-      >>> (fn z => get_run_paction z >>= (fn x => run_action x z))
-      >>> Down4.move >>> Down5.move >>> Down1.move  *)
-      (* >>> run_action *)
-      (* >>> Z.Zippy_DFS.first3 >>> fold_paction *)
-      (* >>> fold_run_max_paction_dfs_halve_prio_depth *)
-      (* >>> Z1.ZM.Zip.move *)
-      (* >>> with_state pretty_gc *)
-      (* >>> with_state pretty_gcs *)
-      (* >>> pretty_actionc *)
-      (* >>> pretty_action *)
-      (* >>> finish_gclusters_oldest_first @{context} >>> arr (Seq.list_of) *)
-      (* >>> finish_promising_gclusters_oldest_first @{context} >>> arr (Seq.list_of) *)
-      )
-      |> (fn f => f (Goal.protect 6 @{thm test}) |> MS.eval @{context})
-      ))
-  end
+  (*syntax setup for monads and arrows*)
+  structure SC = \<^eval>\<open>sfx_ParaT_nargs "Semi_Category"\<close>(Zippy)
+  structure C = \<^eval>\<open>sfx_ParaT_nargs "Category"\<close>(Zippy)
+  structure M = \<^eval>\<open>sfx_ParaT_nargs "Monad"\<close>(Zippy.M)
+  open SC Zippy M
+
+  (*halves the priorities at each pull of an action's result sequence*)
+  fun halve_prio_co p = update_prio_co (fn _ => P.halve) p
+
+  (*add a tactic action whose results' priorites are halved after each pull*)
+  fun add_tac amd p focus tac z =
+    amd >>= (fn amd => cons_move_tac amd (halve_prio_co p) tac focus z)
+
+  (*tactic solving every goal*)
+  fun cheat_tac prog ctxt = Skip_Proof.cheat_tac ctxt
+    |> lift_all_goals_focus_tac (K (Zippy_Result_Metadata.metadata prog))
+    T.single_goal_empty_target
+
+  (*resolution with theorems*)
+  fun zippy_resolve_tac prog thms ctxt = resolve_tac ctxt thms
+    |> lift_every_goals_focus_tac (K (Zippy_Result_Metadata.metadata prog))
+    T.single_goal_moved_target
+
+  (*just some action metadata*)
+  fun amd _ = AMD.metadata (@{binding "test action"}, "action description")
 \<close>
 
-(*
+text \<open>Figure 6 from the paper.
 
-GCS
-|       |
-GC      GC
-|   |    |
-AC  AC   AC
-| |  |    |
-A A  A    A
-|    |    |
-AA   AA   AA
-|    |    |
-GCS  GCS  GCS
+Exhaustively run all rules and apply as tactic. Of course, this is only to show how the zipper
+works and not meant for production. When used in practice, one should return results as soon as
+there are no more subgoals in one of the tree's branches.\<close>
 
-*)
+lemma shows "A \<and> B" "C \<and> D"
+apply (tactic \<open>fn state =>
+  let
+    val amd = amd ()
+    val opt_statesq =
+      (*initialise the zipper*)
+      (init_state' mk_gcd_more state >>= arr snd
+      (*add the conjunction tactic to the first goal cluster*)
+      >>= Down1.move
+      >>= with_state (zippy_resolve_tac RMD.promising @{thms conjI} #> add_tac amd P.HIGH (F.goals [1]))
+      (*add the conjunction tactic to the second goal cluster*)
+      >>= Up4.move >>= Up3.move >>= Z2.ZM.Down.move
+      >>= with_state (zippy_resolve_tac RMD.promising @{thms conjI} #> add_tac amd P.HIGH (F.goals [1]))
+      >>= top4 >>= Z1.ZM.Unzip.move
+      (*repeat best-first-search until no more changes (instead of NONE, you can pass in SOME fuel); cf. below*)
+      >>= repeat_fold_run_max_paction_dfs NONE
+      (*get the theorems*)
+      >>= Z1.ZM.Zip.move >>= with_state finish_gclusters_oldest_first)
+      (*pass context to state monad*)
+      |> MS.eval @{context}
+  in
+    case opt_statesq of
+      NONE => Seq.empty
+    | SOME statesq =>
+        let val _ = Seq.list_of statesq |> @{make_string} |> writeln
+        in statesq end
+  end
+\<close>)
+(*you can backtrack with "back"*)
+back
+back
+back
+oops
+
+declare [[ML_print_depth = 100]]
+
+text \<open>Example with meta variable clusters, navigation, and printing.\<close>
+
+schematic_goal shows "A \<and> ?B" "?B \<and> C" "D"
+ML_val\<open>
+val amd = amd ()
+val state = @{Isar.goal} |> #goal
+val opt_statesq =
+  (*initialise the zipper*)
+  (init_state' mk_gcd_more state >>= arr snd
+  (*print the goal clusters*)
+  >>= (fn z => with_state pretty_gcs z >>= arr Pretty.writeln >>= arr (K z))
+  >>= Down1.move
+  (*print the first goal cluster*)
+  >>= (fn z => with_state pretty_gc z >>= arr Pretty.writeln >>= arr (K z))
+  (*add cheat tac focused on first subgoal of first goal cluster*)
+  >>= with_state (cheat_tac RMD.promising #> add_tac amd P.VERY_HIGH (F.goals [1]))
+  (*print the first action*)
+  >>= (fn z => pretty_action z >>= arr Pretty.writeln >>= arr (K z))
+  >>= Up4.move >>= Up3.move
+  (*add cheat tac focused on second subgoal of first goal cluster*)
+  >>= with_state (cheat_tac RMD.promising #> add_tac amd P.MEDIUM (F.goals [2]))
+  (*print the second action*)
+  >>= (fn z => pretty_action z >>= arr Pretty.writeln >>= arr (K z))
+  >>= Up4.move >>= Up3.move >>= Z2.ZM.Down.move
+  (*print the second goal cluster*)
+  >>= (fn z => with_state pretty_gc z >>= arr Pretty.writeln >>= arr (K z))
+  (*print the local location*)
+  >>= (fn z => L.get (pos2 ()) z >>= arr (@{make_string} #> writeln) >>= arr (K z))
+  (*add cheat tac focused on any subgoal of second goal cluster*)
+  >>= with_state (cheat_tac RMD.promising #> add_tac amd P.LOW F.none)
+  (*print the third action*)
+  >>= (fn z => pretty_action z >>= arr Pretty.writeln >>= arr (K z))
+  >>= top4 >>= Z1.ZM.Unzip.move
+  (*repeat best-first-search for 4 steps*)
+  >>= repeat_fold_run_max_paction_dfs (SOME 4)
+  (*get the theorems*)
+  >>= Z1.ZM.Zip.move >>= with_state finish_gclusters_oldest_first >>= arr Seq.list_of
+  ) |> MS.eval @{context} (*pass context to state monad*)
+\<close>
+oops
 
 end
